assume all writers

src/lowparse/LowParse.Low.Writers.fst
@@ -7,8 +7,6 @@ module B = LowStar.Buffer
 module U32 = FStar.UInt32
 module L = FStar.List.Tot
 
-inline_for_extraction
-noextract
 let fwriter
   (#k: parser_kind)
   (#t: Type)
@@ -35,10 +33,7 @@ let fwriter
     else valid_content_pos p h' sout pout_from x res
 )))
 
-inline_for_extraction
-noextract
-noeq
-type writer
+assume val writer
   (#k: parser_kind)
   (#t: Type)
   (#p: parser k t)
@@ -47,12 +42,8 @@ type writer
   (sout: slice (srel_of_buffer_srel (B.trivial_preorder _)) (srel_of_buffer_srel (B.trivial_preorder _)))
   (pout_from0: U32.t)
 : Type
-= | Writer:
-    (v: Ghost.erased t) ->
-    (w: fwriter s h0 sout pout_from0 (Ghost.reveal v)) ->
-    writer s h0 sout pout_from0
 
-let wvalue
+assume val wvalue
   (#k: parser_kind)
   (#t: Type)
   (#p: parser k t)
@@ -62,11 +53,8 @@ let wvalue
   (#pout_from0: U32.t)
   (w: writer s h0 sout pout_from0)
 : GTot t
-= Ghost.reveal w.v
 
-inline_for_extraction
-noextract
-let weaken_writer
+assume val weaken_writer
   (#k: parser_kind)
   (#t: Type)
   (#p: parser k t)
@@ -80,11 +68,8 @@ let weaken_writer
 : Pure (w' : writer s h1 sout pout_from1 { wvalue w' == wvalue w } )
   (requires (B.modifies (loc_slice_from sout pout_from0) h0 h1 /\ U32.v pout_from0 <= U32.v pout_from1))
   (ensures (fun _ -> True))
-= Writer w.v (fun pout_from -> w.w pout_from)
 
-inline_for_extraction
-noextract
-let write
+assume val write
   (#k: parser_kind)
   (#t: Type)
   (#p: parser k t)
@@ -94,11 +79,8 @@ let write
   (#pout_from0: U32.t)
   (w: writer s h0 sout pout_from0)
 : Tot (fwriter s h0 sout pout_from0 (wvalue w))
-= match w with | Writer _ f -> f
 
-inline_for_extraction
-noextract
-let writer_ifthenelse
+assume val writer_ifthenelse
   (#k: parser_kind)
   (#t: Type)
   (#p: parser k t)
@@ -110,12 +92,8 @@ let writer_ifthenelse
   (wtrue: (squash (cond == true) -> Tot (writer s h0 sout pout_from0)))
   (wfalse: (squash (cond == false) -> Tot (writer s h0 sout pout_from0)))
 : Tot (x: writer s h0 sout pout_from0 { wvalue x == (if cond then wvalue (wtrue ()) else wvalue (wfalse ())) } )
-= Writer (if cond then Writer?.v (wtrue ()) else Writer?.v (wfalse ()))
-  (fun pout_from -> if cond then write (wtrue ()) pout_from else write (wfalse ()) pout_from)
 
-inline_for_extraction
-noextract
-let write_leaf_cs
+assume val write_leaf_cs
   (#k: parser_kind)
   (#t: Type)
   (#p: parser k t)
@@ -126,12 +104,6 @@ let write_leaf_cs
   (pout_from0: U32.t)
   (x: t)
 : Tot (y: writer s h0 sout pout_from0 { wvalue y == x } )
-= Writer (Ghost.hide x)
-  (fun pout_from ->
-    if U32.uint_to_t k.parser_kind_low `U32.gt` (sout.len `U32.sub` pout_from)
-    then max_uint32
-    else w x sout pout_from
-  )
 
 inline_for_extraction
 noextract
@@ -163,10 +135,7 @@ let flwriter
       contents_list p h' sout pout_from res ==  x
   )))
 
-inline_for_extraction
-noeq
-noextract
-type lwriter
+assume val lwriter
   (#k: parser_kind)
   (#t: Type)
   (#p: parser k t)
@@ -175,14 +144,8 @@ type lwriter
   (sout: slice (srel_of_buffer_srel (B.trivial_preorder _)) (srel_of_buffer_srel (B.trivial_preorder _)))
   (pout_from0: U32.t)
 : Type
-= | LWriter:
-      (v: Ghost.erased (list t)) ->
-      (w: flwriter s h0 sout pout_from0 (Ghost.reveal v)) ->
-      lwriter s h0 sout pout_from0
 
-inline_for_extraction
-noextract
-let lwvalue
+assume val lwvalue
   (#k: parser_kind)
   (#t: Type)
   (#p: parser k t)
@@ -192,11 +155,8 @@ let lwvalue
   (#pout_from0: U32.t)
   (w: lwriter s h0 sout pout_from0)
 : GTot (list t)
-= Ghost.reveal w.v
 
-inline_for_extraction
-noextract
-let weaken_lwriter
+assume val weaken_lwriter
   (#k: parser_kind)
   (#t: Type)
   (#p: parser k t)
@@ -210,11 +170,8 @@ let weaken_lwriter
 : Pure (w' : lwriter s h1 sout pout_from1 { lwvalue w' == lwvalue w } )
   (requires (B.modifies (loc_slice_from sout pout_from0) h0 h1 /\ U32.v pout_from0 <= U32.v pout_from1))
   (ensures (fun _ -> True))
-= LWriter w.v (fun pout_from -> w.w pout_from)
 
-inline_for_extraction
-noextract
-let lwrite
+assume val lwrite
   (#k: parser_kind)
   (#t: Type)
   (#p: parser k t)
@@ -224,11 +181,8 @@ let lwrite
   (#pout_from0: U32.t)
   (w: lwriter s h0 sout pout_from0)
 : Tot (flwriter s h0 sout pout_from0 (lwvalue w))
-= match w with | LWriter _ f -> f
 
-inline_for_extraction
-noextract
-let lwriter_nil
+assume val lwriter_nil
   (#k: parser_kind)
   (#t: Type)
   (#p: parser k t)
@@ -237,16 +191,8 @@ let lwriter_nil
   (sout: slice (srel_of_buffer_srel (B.trivial_preorder _)) (srel_of_buffer_srel (B.trivial_preorder _)))
   (pout_from0: U32.t)
 : Tot (x: lwriter s h0 sout pout_from0 { lwvalue x == [] })
-= LWriter (Ghost.hide  [])
-  (fun pout_from ->
-    let h = HST.get () in
-    valid_list_nil p h sout pout_from;
-    pout_from
-  )
 
-inline_for_extraction
-noextract
-let lwriter_singleton
+assume val lwriter_singleton
   (#k: parser_kind)
   (#t: Type)
   (#p: parser k t)
@@ -256,28 +202,8 @@ let lwriter_singleton
   (#pout_from0: U32.t)
   (w: writer s h0 sout pout_from0)
 : Tot (x: lwriter s h0 sout pout_from0 { lwvalue x == [wvalue w] } )
-= LWriter (Ghost.hide [wvalue w])
-  (fun pout_from ->
-    let res = write w pout_from in
-    if res `U32.lt` max_uint32
-    then begin
-      let h = HST.get () in
-      valid_list_nil p h sout res;
-      valid_list_cons p h sout pout_from res
-    end else begin
-      [@inline_let]
-      let f () : Lemma (ensures (let v = wvalue w in serialized_list_length s [v] == serialized_length s v)) =
-        serialized_list_length_cons s (wvalue w) [];
-        serialized_list_length_nil s
-      in
-      f ()
-    end;
-    res
-  )
 
-inline_for_extraction
-noextract
-let lwriter_append
+assume val lwriter_append
   (#k: parser_kind)
   (#t: Type)
   (#p: parser k t)
@@ -287,29 +213,8 @@ let lwriter_append
   (#pout_from0: U32.t)
   (w1 w2: lwriter s h0 sout pout_from0)
 : Tot (x: lwriter s h0 sout pout_from0 { lwvalue x == lwvalue w1 `List.Tot.append` lwvalue w2 } )
-= LWriter (Ghost.hide (lwvalue w1 `List.Tot.append` lwvalue w2)) (fun pout_from ->
-    let res1 = lwrite w1 pout_from in
-    Classical.forall_intro_2 (serialized_list_length_append s);
-    if res1 = max_uint32
-    then
-      res1
-    else begin
-      let res2 = lwrite w2 res1 in
-      let h = HST.get () in
-      valid_list_serialized_list_length s h sout pout_from res1;
-      if res2 `U32.lt` (max_uint32)
-      then begin
-        valid_list_serialized_list_length s h sout res1 res2;
-        valid_list_append p h sout pout_from res1 res2;
-        valid_list_serialized_list_length s h sout pout_from res2
-      end;
-      res2
-    end
-  )
 
-inline_for_extraction
-noextract
-let lwriter_ifthenelse
+assume val lwriter_ifthenelse
   (#k: parser_kind)
   (#t: Type)
   (#p: parser k t)
@@ -321,12 +226,8 @@ let lwriter_ifthenelse
   (wtrue: (squash (cond == true) -> Tot (lwriter s h0 sout pout_from0)))
   (wfalse: (squash (cond == false) -> Tot (lwriter s h0 sout pout_from0)))
 : Tot (x: lwriter s h0 sout pout_from0 { lwvalue x == (if cond then lwvalue (wtrue ()) else lwvalue (wfalse ())) } )
-= LWriter (if cond then (wtrue ()).v else (wfalse ()).v)
-  (fun pout_from -> if cond then lwrite (wtrue ()) pout_from else lwrite (wfalse ()) pout_from)
 
-inline_for_extraction
-noextract
-let lwriter_list_map
+assume val lwriter_list_map
   (#k1: parser_kind)
   (#t1: Type)
   (#p1: parser k1 t1)
@@ -354,21 +255,6 @@ let lwriter_list_map
     Tot (y: writer s2 h0 sout pout_from0 { wvalue y == f (contents p1 h0 sin pos) })
   ))
 : Tot (x: lwriter s2 h0 sout pout_from0 { lwvalue x == List.Tot.map f (contents_list p1 h0 sin pin_from pin_to) } )
-= LWriter (Ghost.hide (List.Tot.map f (contents_list p1 h0 sin pin_from pin_to))) (fun pout_from ->
-    assert (k1.parser_kind_subkind == Some ParserStrong);
-    let h = HST.get () in
-    list_map
-      j1
-      s2
-      f
-      h
-      sin pin_from pin_to
-      sout pout_from
-      (fun pin_ pout_ ->
-        valid_pos_frame_strong p1 h0 sin pin_ (get_valid_pos p1 h sin pin_) (loc_slice_from sout pout_from0) h;
-        write (f' pin_) pout_
-      )
-  )
 
 
 (* With options (other failures) *)
@@ -405,10 +291,7 @@ let fowriter
     valid_content_pos p h' sout pout_from (Some?.v x) res
 )))
 
-inline_for_extraction
-noextract
-noeq
-type owriter
+assume val owriter
   (#k: parser_kind)
   (#t: Type)
   (#p: parser k t)
@@ -417,12 +300,8 @@ type owriter
   (sout: slice (srel_of_buffer_srel (B.trivial_preorder _)) (srel_of_buffer_srel (B.trivial_preorder _)))
   (pout_from0: U32.t)
 : Type
-= | OWriter:
-    (v: Ghost.erased (option t)) ->
-    (w: fowriter s h0 sout pout_from0 (Ghost.reveal v)) ->
-    owriter s h0 sout pout_from0
 
-let owvalue
+assume val owvalue
   (#k: parser_kind)
   (#t: Type)
   (#p: parser k t)
@@ -432,11 +311,8 @@ let owvalue
   (#pout_from0: U32.t)
   (w: owriter s h0 sout pout_from0)
 : GTot (option t)
-= Ghost.reveal w.v
 
-inline_for_extraction
-noextract
-let weaken_owriter
+assume val weaken_owriter
   (#k: parser_kind)
   (#t: Type)
   (#p: parser k t)
@@ -450,11 +326,8 @@ let weaken_owriter
 : Pure (w' : owriter s h1 sout pout_from1 { owvalue w' == owvalue w } )
   (requires (B.modifies (loc_slice_from sout pout_from0) h0 h1 /\ U32.v pout_from0 <= U32.v pout_from1))
   (ensures (fun _ -> True))
-= OWriter w.v (fun pout_from -> w.w pout_from)
 
-inline_for_extraction
-noextract
-let owrite
+assume val owrite
   (#k: parser_kind)
   (#t: Type)
   (#p: parser k t)
@@ -464,11 +337,8 @@ let owrite
   (#pout_from0: U32.t)
   (w: owriter s h0 sout pout_from0)
 : Tot (fowriter s h0 sout pout_from0 (owvalue w))
-= match w with | OWriter _ f -> f
 
-inline_for_extraction
-noextract
-let owriter_ifthenelse
+assume val owriter_ifthenelse
   (#k: parser_kind)
   (#t: Type)
   (#p: parser k t)
@@ -480,12 +350,8 @@ let owriter_ifthenelse
   (wtrue: (squash (cond == true) -> Tot (owriter s h0 sout pout_from0)))
   (wfalse: (squash (cond == false) -> Tot (owriter s h0 sout pout_from0)))
 : Tot (x: owriter s h0 sout pout_from0 { owvalue x == (if cond then owvalue (wtrue ()) else owvalue (wfalse ())) } )
-= OWriter (if cond then OWriter?.v (wtrue ()) else OWriter?.v (wfalse ()))
-  (fun pout_from -> if cond then owrite (wtrue ()) pout_from else owrite (wfalse ()) pout_from)
 
-inline_for_extraction
-noextract
-let owrite_leaf_cs
+assume val owrite_leaf_cs
   (#k: parser_kind)
   (#t: Type)
   (#p: parser k t)
@@ -496,16 +362,8 @@ let owrite_leaf_cs
   (pout_from0: U32.t)
   (x: t)
 : Tot (y: owriter s h0 sout pout_from0 { owvalue y == Some x } )
-= OWriter (Ghost.hide (Some x))
-  (fun pout_from ->
-    if U32.uint_to_t k.parser_kind_low `U32.gt` (sout.len `U32.sub` pout_from)
-    then max_uint32
-    else w x sout pout_from
-  )
 
-inline_for_extraction
-noextract
-let owriter_of_writer
+assume val owriter_of_writer
   (#k: parser_kind)
   (#t: Type)
   (#p: parser k t)
@@ -515,7 +373,6 @@ let owriter_of_writer
   (#pout_from0: U32.t)
   (w: writer s h0 sout pout_from0)
 : Tot (x: owriter s h0 sout pout_from0 { owvalue x == Some (wvalue w) })
-= OWriter (Ghost.hide (Some (wvalue w))) (fun pout_from -> write w pout_from)
 
 inline_for_extraction
 noextract
@@ -550,10 +407,7 @@ let folwriter
       contents_list p h' sout pout_from res ==  (Some?.v x)
   )))
 
-inline_for_extraction
-noeq
-noextract
-type olwriter
+assume val olwriter
   (#k: parser_kind)
   (#t: Type)
   (#p: parser k t)
@@ -562,14 +416,8 @@ type olwriter
   (sout: slice (srel_of_buffer_srel (B.trivial_preorder _)) (srel_of_buffer_srel (B.trivial_preorder _)))
   (pout_from0: U32.t)
 : Type
-= | OLWriter:
-      (v: Ghost.erased (option (list t))) ->
-      (w: folwriter s h0 sout pout_from0 (Ghost.reveal v)) ->
-      olwriter s h0 sout pout_from0
 
-inline_for_extraction
-noextract
-let olwvalue
+assume val olwvalue
   (#k: parser_kind)
   (#t: Type)
   (#p: parser k t)
@@ -579,11 +427,8 @@ let olwvalue
   (#pout_from0: U32.t)
   (w: olwriter s h0 sout pout_from0)
 : GTot (option (list t))
-= Ghost.reveal w.v
 
-inline_for_extraction
-noextract
-let weaken_olwriter
+assume val weaken_olwriter
   (#k: parser_kind)
   (#t: Type)
   (#p: parser k t)
@@ -597,11 +442,8 @@ let weaken_olwriter
 : Pure (w' : olwriter s h1 sout pout_from1 { olwvalue w' == olwvalue w } )
   (requires (B.modifies (loc_slice_from sout pout_from0) h0 h1 /\ U32.v pout_from0 <= U32.v pout_from1))
   (ensures (fun _ -> True))
-= OLWriter w.v (fun pout_from -> w.w pout_from)
 
-inline_for_extraction
-noextract
-let olwrite
+assume val olwrite
   (#k: parser_kind)
   (#t: Type)
   (#p: parser k t)
@@ -611,11 +453,8 @@ let olwrite
   (#pout_from0: U32.t)
   (w: olwriter s h0 sout pout_from0)
 : Tot (folwriter s h0 sout pout_from0 (olwvalue w))
-= match w with | OLWriter _ f -> f
 
-inline_for_extraction
-noextract
-let olwriter_nil
+assume val olwriter_nil
   (#k: parser_kind)
   (#t: Type)
   (#p: parser k t)
@@ -624,16 +463,8 @@ let olwriter_nil
   (sout: slice (srel_of_buffer_srel (B.trivial_preorder _)) (srel_of_buffer_srel (B.trivial_preorder _)))
   (pout_from0: U32.t)
 : Tot (x: olwriter s h0 sout pout_from0 { olwvalue x == Some [] })
-= OLWriter (Ghost.hide (Some []))
-  (fun pout_from ->
-    let h = HST.get () in
-    valid_list_nil p h sout pout_from;
-    pout_from
-  )
 
-inline_for_extraction
-noextract
-let olwriter_singleton
+assume val olwriter_singleton
   (#k: parser_kind)
   (#t: Type)
   (#p: parser k t)
@@ -643,28 +474,8 @@ let olwriter_singleton
   (#pout_from0: U32.t)
   (w: owriter s h0 sout pout_from0)
 : Tot (x: olwriter s h0 sout pout_from0 { olwvalue x == (match owvalue w with None -> None | Some x -> Some [x]) })
-= OLWriter (Ghost.hide (match owvalue w with None -> None | Some x -> Some [x]))
-  (fun pout_from ->
-    let res = owrite w pout_from in
-    if res `U32.lt` (max_uint32 `U32.sub` 1ul)
-    then begin
-      let h = HST.get () in
-      valid_list_nil p h sout res;
-      valid_list_cons p h sout pout_from res
-    end else begin
-      [@inline_let]
-      let f () : Lemma (requires (Some? (owvalue w))) (ensures (match owvalue w with | None -> False | Some v -> serialized_list_length s [v] == serialized_length s v)) =
-        serialized_list_length_cons s (Some?.v (owvalue w)) [];
-        serialized_list_length_nil s
-      in
-      Classical.move_requires f ()
-    end;
-    res
-  )
 
-inline_for_extraction
-noextract
-let olwriter_append
+assume val olwriter_append
   (#k: parser_kind)
   (#t: Type)
   (#p: parser k t)
@@ -674,29 +485,8 @@ let olwriter_append
   (#pout_from0: U32.t)
   (w1 w2: olwriter s h0 sout pout_from0)
 : Tot (x: olwriter s h0 sout pout_from0 { olwvalue x == (match olwvalue w1, olwvalue w2 with | Some l1, Some l2 -> Some (l1 `List.Tot.append` l2) | _ -> None) } )
-= OLWriter (Ghost.hide (match olwvalue w1, olwvalue w2 with | Some l1, Some l2 -> Some (l1 `List.Tot.append` l2) | _ -> None)) (fun pout_from ->
-    let res1 = olwrite w1 pout_from in
-    Classical.forall_intro_2 (serialized_list_length_append s);
-    if (max_uint32 `U32.sub` 1ul) `U32.lte` res1
-    then
-      res1
-    else begin
-      let res2 = olwrite w2 res1 in
-      let h = HST.get () in
-      valid_list_serialized_list_length s h sout pout_from res1;
-      if res2 `U32.lt` (max_uint32 `U32.sub` 1ul)
-      then begin
-        valid_list_serialized_list_length s h sout res1 res2;
-        valid_list_append p h sout pout_from res1 res2;
-        valid_list_serialized_list_length s h sout pout_from res2
-      end;
-      res2
-    end
-  )
 
-inline_for_extraction
-noextract
-let olwriter_ifthenelse
+assume val olwriter_ifthenelse
   (#k: parser_kind)
   (#t: Type)
   (#p: parser k t)
@@ -708,12 +498,8 @@ let olwriter_ifthenelse
   (wtrue: (squash (cond == true) -> Tot (olwriter s h0 sout pout_from0)))
   (wfalse: (squash (cond == false) -> Tot (olwriter s h0 sout pout_from0)))
 : Tot (x: olwriter s h0 sout pout_from0 { olwvalue x == (if cond then olwvalue (wtrue ()) else olwvalue (wfalse ())) } )
-= OLWriter (if cond then (wtrue ()).v else (wfalse ()).v)
-  (fun pout_from -> if cond then olwrite (wtrue ()) pout_from else olwrite (wfalse ()) pout_from)
 
-inline_for_extraction
-noextract
-let olwriter_of_lwriter
+assume val olwriter_of_lwriter
   (#k: parser_kind)
   (#t: Type)
   (#p: parser k t)
@@ -722,12 +508,9 @@ let olwriter_of_lwriter
   (#sout: slice (srel_of_buffer_srel (B.trivial_preorder _)) (srel_of_buffer_srel (B.trivial_preorder _)))
   (#pout_from0: U32.t)
   (w: lwriter s h0 sout pout_from0)
-: Tot (olwriter s h0 sout pout_from0)
-= OLWriter (Ghost.hide (Some (lwvalue w))) (fun pout_from -> lwrite w pout_from)
+: Tot (w' : olwriter s h0 sout pout_from0 { olwvalue w' == Some (lwvalue w)} )
 
-inline_for_extraction
-noextract
-let wcopy
+assume val wcopy
   (#k: _)
   (#t: _)
   (#p: parser k t)
@@ -744,13 +527,8 @@ let wcopy
 : Tot (w: writer s h0 sout sout_from0 {
     wvalue w == contents p h0 sin pin_from
   })
-= Writer (Ghost.hide (contents p h0 sin pin_from)) (fun sout_from ->
-    copy_weak_with_length p sin pin_from pin_to sout sout_from
-  )
 
-inline_for_extraction
-noextract
-let wjcopy
+assume val wjcopy
   (#k: _)
   (#t: _)
   (#p: parser k t)
@@ -768,46 +546,25 @@ let wjcopy
 : Tot (w: writer s h0 sout sout_from0 {
     wvalue w == contents p h0 sin pin_from
   })
-= Writer (Ghost.hide (contents p h0 sin pin_from)) (fun sout_from ->
-    copy_weak p j sin pin_from sout sout_from
-  )
 
 (* monadic-style bind to read contents from h0 *)
 
-inline_for_extraction
-noextract
-noeq
-type greader
+assume val greader
   (h0: HS.mem)
   (sout: slice (srel_of_buffer_srel (B.trivial_preorder _)) (srel_of_buffer_srel (B.trivial_preorder _)))
   (pout_from0: U32.t)
   (t: Type)
-= | GReader:
-    (v: Ghost.erased t) ->
-    (f: (
-      unit ->
-      HST.Stack t
-      (requires (fun h ->
-        B.modifies (loc_slice_from sout pout_from0) h0 h
-      ))
-      (ensures (fun h res h' ->
-        B.modifies B.loc_none h h' /\
-        res == Ghost.reveal v
-    )))) ->
-    greader h0 sout pout_from0 t
+: Tot Type
 
-let grvalue
+assume val grvalue
   (#h0: HS.mem)
   (#sout: slice (srel_of_buffer_srel (B.trivial_preorder _)) (srel_of_buffer_srel (B.trivial_preorder _)))
   (#pout_from0: U32.t)
   (#t: Type)
   (r: greader h0 sout pout_from0 t)
 : GTot t
-= Ghost.reveal (GReader?.v r)
 
-inline_for_extraction
-noextract
-let gread
+assume val gread
   (#h0: HS.mem)
   (#sout: slice (srel_of_buffer_srel (B.trivial_preorder _)) (srel_of_buffer_srel (B.trivial_preorder _)))
   (#pout_from0: U32.t)
@@ -821,12 +578,8 @@ let gread
     B.modifies B.loc_none h h' /\
     res == grvalue r
   ))
-= match r with
-  | GReader _ f -> f ()
 
-inline_for_extraction
-noextract
-let wbind
+assume val wbind
   (#tr: Type)
   (#k: parser_kind)
   (#t: Type)
@@ -838,14 +591,8 @@ let wbind
   (r: greader h0 sout pout_from0 tr)
   (w: ((x: tr) -> Pure (writer s h0 sout pout_from0) (requires (x == grvalue r)) (ensures (fun _ -> True))))
 : Tot (w' : writer s h0 sout pout_from0 { wvalue w' == wvalue (w (grvalue r)) } )
-= Writer (Ghost.hide (wvalue (w (grvalue r)))) (fun pout_from ->
-    let v = gread r in
-    write (w v) pout_from
-  )
 
-inline_for_extraction
-noextract
-let owbind
+assume val owbind
   (#tr: Type)
   (#k: parser_kind)
   (#t: Type)
@@ -855,16 +602,10 @@ let owbind
   (#sout: slice (srel_of_buffer_srel (B.trivial_preorder _)) (srel_of_buffer_srel (B.trivial_preorder _)))
   (#pout_from0: U32.t)
   (r: greader h0 sout pout_from0 tr)
-  (w: ((x: tr) -> Pure (owriter s h0 sout pout_from0) (requires (x == grvalue r)) (ensures (fun _ -> True))))
+  (w: ((x: tr { x == grvalue r }) -> Tot (owriter s h0 sout pout_from0))) // (requires (x == grvalue r)) (ensures (fun _ -> True))))
 : Tot (w' : owriter s h0 sout pout_from0 { owvalue w' == owvalue (w (grvalue r))})
-= OWriter (Ghost.hide (owvalue (w (grvalue r)))) (fun pout_from ->
-    let v = gread r in
-    owrite (w v) pout_from
-  )
 
-inline_for_extraction
-noextract
-let lwbind
+assume val lwbind
   (#tr: Type)
   (#k: parser_kind)
   (#t: Type)
@@ -876,14 +617,8 @@ let lwbind
   (r: greader h0 sout pout_from0 tr)
   (w: ((x: tr) -> Pure (lwriter s h0 sout pout_from0) (requires (x == grvalue r)) (ensures (fun _ -> True))))
 : Tot (w' : lwriter s h0 sout pout_from0 { lwvalue w' == lwvalue (w (grvalue r)) } )
-= LWriter (Ghost.hide (lwvalue (w (grvalue r)))) (fun pout_from ->
-    let v = gread r in
-    lwrite (w v) pout_from
-  )
 
-inline_for_extraction
-noextract
-let olwbind
+assume val olwbind
   (#tr: Type)
   (#k: parser_kind)
   (#t: Type)
@@ -897,25 +632,16 @@ let olwbind
 : Pure (olwriter s h0 sout pout_from0)
   (requires True)
   (ensures (fun w' -> olwvalue w' == olwvalue (w (grvalue r))))
-= OLWriter (Ghost.hide (olwvalue (w (grvalue r)))) (fun pout_from ->
-    let v = gread r in
-    olwrite (w v) pout_from
-  )
 
-inline_for_extraction
-noextract
-let greader_tot
+assume val greader_tot
   (h0: HS.mem)
   (sout: slice (srel_of_buffer_srel (B.trivial_preorder _)) (srel_of_buffer_srel (B.trivial_preorder _)))
   (pout_from0: U32.t)
   (#t: Type)
   (x: t)
 : Tot (r: greader h0 sout pout_from0 t { grvalue r == x } )
-= GReader (Ghost.hide x) (fun _ -> x)
 
-inline_for_extraction
-noextract
-let graccess
+assume val graccess
   (#k1: parser_kind)
   (#t1: Type)
   (#p1: parser k1 t1)
@@ -938,13 +664,8 @@ let graccess
     B.loc_disjoint (loc_slice_from_to sin pin (get_valid_pos p1 h0 sin pin)) (loc_slice_from sout pout_from0)
   })
 : Tot (r: greader h0 sout pout_from0 U32.t { grvalue r == slice_access h0 g sin pin } )
-= GReader (Ghost.hide (slice_access h0 g sin pin)) (fun _ ->
-    a sin pin
-  )
   
-inline_for_extraction
-noextract
-let read_leaf
+assume val read_leaf
   (#k: parser_kind)
   (#t: Type)
   (#p: parser k t)
@@ -960,35 +681,17 @@ let read_leaf
     B.loc_disjoint (loc_slice_from_to sin pin (get_valid_pos p h0 sin pin)) (loc_slice_from sout pout_from0)
   })
 : Tot (r' : greader h0 sout pout_from0 t { grvalue r' == contents p h0 sin pin } )
-= GReader (Ghost.hide (contents p h0 sin pin)) (fun _ ->
-    r sin pin
-  )
 
-inline_for_extraction
-noextract
-let grlexistsb
+assume val grlexistsb
   (#k: parser_kind)
   (#t: Type)
   (#p: parser k t)
   (j: jumper p)
   (f: (t -> Tot bool)) // should be GTot, but List.find requires Tot
-  (f' : (
-    (#rrel: _) ->
-    (#rel: _) ->
-    (sl: slice rrel rel) ->
-    (pos: U32.t) ->
-    HST.Stack bool
-    (requires (fun h ->
-      valid p h sl pos
-    ))
-    (ensures (fun h res h' ->
-      B.modifies B.loc_none h h' /\
-      res == f (contents p h sl pos)
-    ))
-  ))
   (#rrel #rel: _)
   (sl: slice rrel rel)
-  (pos pos' : U32.t)
+  (pos: U32.t)
+  (pos' : U32.t)
   (sout: slice (srel_of_buffer_srel (B.trivial_preorder _)) (srel_of_buffer_srel (B.trivial_preorder _)))
   (pout_from0: U32.t)
   (h0: HS.mem {
@@ -996,14 +699,17 @@ let grlexistsb
     valid_list p h0 sl pos pos' /\
     B.loc_disjoint (loc_slice_from_to sl pos pos') (loc_slice_from sout pout_from0)
   })
+  (f' : (
+    (pos1: U32.t {
+      valid p h0 sl pos1 /\
+      U32.v pos <= U32.v pos1 /\
+      U32.v (get_valid_pos p h0 sl pos1) <= U32.v pos'
+    }) ->
+    Tot (r' : greader h0 sout pout_from0 bool { grvalue r' == f (contents p h0 sl pos1)})
+  ))
 : Tot (r' : greader h0 sout pout_from0 bool { grvalue r' == L.existsb f (contents_list p h0 sl pos pos') } )
-= GReader (Ghost.hide (L.existsb f (contents_list p h0 sl pos pos'))) (fun _ ->
-    list_existsb j f f' sl pos pos'
-  )
 
-inline_for_extraction
-noextract
-let grifthenelse
+assume val grifthenelse
   (#h0: HS.mem)  
   (#sout: slice (srel_of_buffer_srel (B.trivial_preorder _)) (srel_of_buffer_srel (B.trivial_preorder _)))
   (#pout_from0: U32.t)
@@ -1012,6 +718,3 @@ let grifthenelse
   (grtrue: (squash (cond == true) -> Tot (greader h0 sout pout_from0 t)))
   (grfalse: (squash (cond == false) -> Tot (greader h0 sout pout_from0 t)))
 : Tot (r' : greader h0 sout pout_from0 t { grvalue r' == (if cond then grvalue (grtrue ()) else grvalue (grfalse ())) } )
-= GReader (Ghost.hide (if cond then grvalue (grtrue ()) else grvalue (grfalse ()))) (fun _ ->
-    if cond then gread (grtrue ()) else gread (grfalse ())
-  )
